translator/monadic/ml_monad_translator_interfaceLib.sml
@@ -21,8 +21,8 @@ val _ = monadsyntax.temp_add_monadsyntax()
 
 (* Parser overloadings *)
 val _ = temp_overload_on ("monad_bind", ``st_ex_bind``);
-val _ = temp_overload_on ("monad_unitbind", ``\x y. st_ex_bind x (\z. y)``);
-val _ = temp_overload_on ("monad_ignore_bind", ``\x y. st_ex_bind x (\z. y)``);
+val _ = temp_overload_on ("monad_unitbind", ``st_ex_ignore_bind``);
+val _ = temp_overload_on ("monad_ignore_bind", ``st_ex_ignore_bind``);
 val _ = temp_overload_on ("return", ``st_ex_return``);
 
 (* Hide "state" due to semanticPrimitives *)
@@ -528,22 +528,16 @@ local
     `∀  f : 'b -> 'a -> ('d, 'c) exc # 'a .
       f = ( λ x s . f x s)`,
       metis_tac[ETA_THM]
-  )
-
-  val monad_state_if = Q.prove (
-    `∀ b f g x .
-      (λ s . if b then f s else g s) = (λ s . (if b then f else g) s)`,
-    fs[Once COND_RATOR]
   );
 
-  val monad_state_let = Q.prove (
-    `∀ n m .
-      (λ s . let x = n in (m s)) = (λ s . (let x = n in m) s)`,
-    fs[]
+  val ignore_st_ex_eta_intro = Q.prove(
+    `∀  f : 'a -> ('d, 'c) exc # 'a .
+      f = ( λ s . f s)`,
+      fs[ETA_THM]
   );
 
-  val remove_state_arg = Q.prove (
-    `∀ f g . (∀ s . (f s = g s)) ⇔ (f = λ a . g a)`,
+  val remove_state_arg = Q.prove(
+    `∀ f:'a -> ('b, 'c) exc # 'a  g . (∀ s . (f s = g s)) ⇔ (f = λ a . g a)`,
     rw[] >>
     EQ_TAC >>
     rw[] >>
@@ -552,41 +546,70 @@ local
 
   (* Theorems to push/pull state term into compound terms *)
   (* TODO - add more theorems, these will not be enough *)
-  val pull_thms = [monad_state_if, monad_state_let]
-  val push_thms = List.map GSYM pull_thms
+  val push_thms = [
+                   COND_RATOR |> INST_TYPE [beta |-> ``:('b, 'c) exc # 'a``],
+                   LET_RATOR |> INST_TYPE [gamma |-> ``:('c, 'd) exc # 'b``],
+                   literal_case_RATOR |>
+                      INST_TYPE [gamma |-> ``:('c, 'd) exc # 'b``],
+                   LET2_RATOR |> INST_TYPE [gamma |-> ``:('c, 'd) exc # 'b``]
+                   ]
+  val pull_thms = List.map GSYM push_thms
 
   val st_ex_bind_term = (fetch "ml_monadBase" "st_ex_bind_def" |> concl |>
     dest_forall |> snd |> dest_forall |> snd |> lhs |> strip_comb |> fst)
+  val st_ex_ignore_bind_term = (fetch "ml_monadBase" "st_ex_ignore_bind_def") |>
+    concl |> dest_forall |> snd |> dest_forall |> snd |> lhs |>
+    strip_comb |> fst
 
   (*
    *  Find all ``st_ex_bind x (λ ret . f ret)`` and eta-expand to include the
    *  state, giving ``st_ex_bind x (λ ret state . f ret state)``.
    *  Some extra machinery with bound vars is needed to ensure names end up
-   *  as the user defined originally. Also introduce an explicit state arg.
+   *  as the user defined originally, and that each "state" abstraction has a
+   *  different name. Also introduce an explicit state arg.
    *  Needed so that TotalDefn gives correct termination conditions.
    *)
   fun expand_term tm =
     let val bind_terms =
-          find_terms (fn t => can (match_term ``^st_ex_bind_term x f``) t) tm
+          find_terms
+            (fn t => can (match_term ``^st_ex_bind_term x f``) t) tm
         fun get_bvar_name tm = strip_comb tm |> snd |> last |> bvar |>
                                dest_var |> fst
         val bvar_names = List.map get_bvar_name bind_terms
-        val bvars_binds = Lib.zip bvar_names bind_terms
+        val bind_indexes = List.tabulate(length bind_terms, I)
+        val bvars_binds = Lib.zip bind_indexes (Lib.zip bvar_names bind_terms)
         val bind_terms' = bvars_binds |>
           List.map
-            (fn (bvar, term) => term |>
+            (fn (index, (bvar, term)) => term |>
                     (PAT_CONV ``λ f . ^st_ex_bind_term x f``
                       (ONCE_REWRITE_CONV [st_ex_eta_intro])
               THENC (DEPTH_CONV BETA_CONV)
               THENC (REWRITE_CONV push_thms)
-              THENC (DEPTH_CONV ETA_CONV)
-              THENC (RAND_CONV (RENAME_VARS_CONV [bvar]))
+              THENC (RAND_CONV
+                (RENAME_VARS_CONV [bvar, "sb" ^ int_to_string index]))
+              )
+            )
+
+        val ignore_bind_terms =
+          find_terms
+            (fn t => can (match_term ``^st_ex_ignore_bind_term x f``) t) tm
+        val ignore_bind_indexes = List.tabulate(length ignore_bind_terms, I)
+        val indexes_ignore_binds = Lib.zip ignore_bind_indexes ignore_bind_terms
+        val ignore_bind_terms' = indexes_ignore_binds |>
+          List.map
+            (fn (index, term) => term |>
+                    (PAT_CONV ``λ f . ^st_ex_ignore_bind_term x f``
+                      (ONCE_REWRITE_CONV [ignore_st_ex_eta_intro])
+              THENC (DEPTH_CONV BETA_CONV)
+              THENC (REWRITE_CONV push_thms)
+              THENC (RAND_CONV (RENAME_VARS_CONV ["si" ^ int_to_string index]))
               )
             )
     in tm |> (
-        REWRITE_CONV (bind_terms')
+        REWRITE_CONV (bind_terms' @ ignore_bind_terms')
         THENC RAND_CONV (ONCE_REWRITE_CONV [GSYM ETA_THM])
         THENC REWRITE_CONV [GSYM remove_state_arg]
+        THENC REWRITE_CONV push_thms
       ) |> concl |> rhs |> dest_forall |> snd
     end
 
@@ -595,11 +618,19 @@ local
    *  return to the user. Should in fact give a definition which looks exactly
    *  like the quotation from user input.
    *)
-  fun contract_def def = def |>
-    REWRITE_RULE pull_thms |>
-    CONV_RULE (DEPTH_CONV ETA_CONV) |>
-    REWRITE_RULE [remove_state_arg] |>
-    REWRITE_RULE [ETA_THM]
+  fun contract_def def =
+    let val state_arg =
+          def |> concl |> strip_forall |> snd |> lhs |>
+          strip_comb |> snd |> List.last
+    in
+      def |>
+      REWRITE_RULE pull_thms |>
+      CONV_RULE (DEPTH_CONV ETA_CONV) |>
+      SPEC_ALL |> GEN state_arg |>
+      REWRITE_RULE [remove_state_arg] |>
+      GEN_ALL |>
+      REWRITE_RULE [ETA_THM]
+    end
 
   fun delete_defn name = (
     delete_binding (name ^ (!Defn.def_suffix));
